\documentclass[11pt, a4paper]{article}
\usepackage[utf8]{inputenc}
\usepackage[T1]{fontenc}
\usepackage[francais]{babel}
\usepackage{lmodern}
\usepackage{amsmath}
\usepackage{amssymb}
\usepackage{amsthm}
\input{../../../newcommands.tex}
\begin{document}
\title{Exercise 7}
\author{David Wiedemann}
\maketitle
We will use, without proof, the identity 
\begin{align*}
	\sum_{d|n}^{ } d M( d,r) = r^{d}\\
\end{align*}
First, notice that the left hand side expands to
\begin{align*}
	\frac{rz}{1-rz} &= \sum_{i=1}^{ \infty } ( rz) ^{i}\\
			&= rz + ( rz) ^{2} + ( rz) ^{3} + \ldots\\
			&= rz + r^{2}z^{2} + r^{3}z^{3}
\end{align*}
We will now develop the right hand side and show the equality:
\begin{align}
	\sum_{n=1}^{ \infty } n M( n,r)  \frac{z^{n}}{1-z^{n}} &= \sum_{n=1}^{ \infty } n M( n,r) \sum_{i=1}^{ \infty } z^{ni}\nonumber\\
							       &= \sum_{n=1}^{ \infty } \sum_{i=1}^{ \infty } n M( n,r) z^{ni} \label{eq1}
\end{align}
Notice that, for each integer $k \in \mathbb{N}_{ \geq 1} $, for a fixed $n$, the coefficient of $x^{k}$ in
\[ 
	\sum_{i=1}^{ \infty } n M( n,r) z^{ni}
\]
is 1 if and only if $n|k$.\\
Hence, we can rewrite   (\ref{eq1}) as 
\begin{align*}
\sum_{n=1}^{ \infty } \sum_{d|n}^{ } d M( d,r)  z^{n} &= \sum_{n=1}^{ \infty } r^{n} z^{n}
\end{align*}
This proves the equality.







\end{document}
